src/PlutusIR/Semantics/SemanticEquivalence/Validator.v
@@ -1,0 +1,64 @@
+From PlutusCert Require Import PlutusIR.
+From PlutusCert Require Import PlutusIR.Semantics.Static.Typing.
+From PlutusCert Require Import PlutusIR.Semantics.Dynamic.Bigstep.
+
+Require Import Lists.List.
+Import ListNotations.
+
+Definition eval' t r := exists j, eval t r j.
+Definition succeeds t r := eval' t r /\ value r.
+Notation "t '==>' r" := (eval' t r) (at level 20).
+Notation "t '==>e'" := (exists T, eval' t (Error T)) (at level 20).
+
+Definition val_unit : term :=
+  Constant (ValueOf DefaultUniUnit tt)
+.
+
+Definition ty_validator : ty :=
+  Ty_Fun
+    (Ty_Builtin DefaultUniData)
+    (Ty_Builtin DefaultUniUnit)
+.
+
+Definition validator_equivalent s t :=
+  ([],, [] |-+ s : ty_validator) /\
+  ([],, [] |-+ t : ty_validator) /\
+  forall (d : Data) i,
+    i = Constant (ValueOf DefaultUniData d) ->
+      (Apply s i ==> val_unit <-> Apply t i ==> val_unit) /\
+      (Apply s i ==>e <-> Apply t i ==>e)
+.
+
+Notation "s '=val' t" := (validator_equivalent s t)
+  ( at level 70
+  , no associativity).
+
+Lemma validator_value t r :
+  [],, [] |-+ t : ty_validator ->
+  t ==> r ->
+  r = val_unit \/ is_error r.
+Proof.
+(* TODO: follows from type preservation and result *)
+Admitted.
+
+Module Equivalence.
+
+  Lemma refl t : [] ,, [] |-+ t : ty_validator -> t =val t.
+  Proof.
+    unfold validator_equivalent.
+    intuition.
+  Qed.
+
+  Lemma sym s t : s =val t -> t =val s.
+  Proof.
+    unfold validator_equivalent.
+    intuition.
+  Qed.
+
+  Lemma trans s t u : s =val t -> t =val u -> s =val u.
+  Proof.
+    unfold validator_equivalent.
+    intuition.
+  Qed.
+
+End Equivalence.
